---
title: "Biostat 202B Homework 2"
subtitle: Due April 18, 2024 @ 11:59PM
author: Hanbei Xiong 605257780
format:
  html:
    theme: cosmo
    embed-resources: true
    number-sections: false
    toc: true
    toc-depth: 4
    toc-location: left
    code-fold: false
knitr:
  opts_chunk: 
    cache: false    
    echo: true
    fig.align: 'center'
    fig.width: 6
    fig.height: 4
    message: FALSE
---

# Question 1

![](images/WeChatbb0d8fc93d416fb444a789bb25004e96.png)

**Answer:**

```{=tex}
\begin{align*}
nS_{n}^2 &= \sum_{i=1}^{n} (X_i-\bar{X})^2 \\
&= \sum_{i=1}^{n} ((X_i-\mu)-(\bar{X}-\mu))^2 \\
&= \sum_{i=1}^{n} ((X_i-\mu)^2 - 2(X_i-\mu)(\bar{X}-\mu) + (\bar{X}-\mu)^2) \\
&= \sum_{i=1}^{n} (X_i-\mu)^2 - 2(\bar{X}-\mu)\sum_{i=1}^{n} (X_i-\mu) + n(\bar{X}-\mu)^2 \\
&= \sum_{i=1}^{n} (X_i-\mu)^2 - 2n(\bar{X}-\mu)^2 + n(\bar{X}-\mu)^2 \\
&= \sum_{i=1}^{n} (X_i-\mu)^2 - n(\bar{X}-\mu)^2
\end{align*}
```
Hence, $S_n^2=\frac{1}{n}\sum_{i=1}^{n} (X_i-\mu)^2 - (\bar{X}-\mu)^2$

Let $Y_i=(X_i-\mu)^2$, then $E(Y_i)=\mu_y=\sigma^2$

$Var(Y_i)=E(X_i-\mu)^4-\{E(X_i-\mu)^2\}^2=E(X_i-\mu_x)^4-\sigma^4$

Since $\gamma = \frac{E(X_i-\mu_x)^4}{\sigma^4}$

$Var(Y_i)=\sigma^4(\gamma-1)$

$S_n^2=\frac{1}{n}\sum_{i=1}^{n} Y_i - (\bar{X}-\mu)^2=\bar{Y}-(\bar{X}-\mu)^2$

Consider $\sqrt{n}(S_n^2-\sigma_x^2)=\sqrt{n}\{\bar{Y}-(\bar{X}-\mu)^2-\sigma_x^2\}=\sqrt{n}\{\bar{Y}-(\bar{X}-\mu)^2-\mu_y\}=\sqrt{n}(\bar{Y}-\mu_y)-\sqrt{n}(\bar{X}-\mu)^2$

By CLT, $\sqrt{n}(\bar{Y}-\mu_y)\overset{D}{\rightarrow}\sigma_yZ\sim N(0,\sigma_y^2)$

By CLT, $\sqrt{n}(\bar{X}-\mu)\overset{D}{\rightarrow}N(0,\sigma^2)$

By slutsky, $\bar{X}-\mu = \frac{1}{\sqrt{n}}\sqrt{n}(\bar{X}-\mu)\overset{P}{\rightarrow}0$

By C.M.T, $\sqrt{n}(S_n^2-\sigma_x^2)\overset{D}{\rightarrow}N(0,\sigma^4(\gamma-1))$

# Question 2

![](images/WeChat8a7218fa5d43ec3b02de109635fb06a6.png)

**Answer:**

Since $\frac{1}{\sqrt{n}}\rightarrow 0$ as $n\rightarrow \infty$, we have

$Y_n-\theta \rightarrow 0$ as $n\rightarrow \infty$.

$Y_n\rightarrow \theta$ in probability. (Note: There is a typo in the question)

# Question 3

![](images/WeChatcf6436f715fc94561dd3e0347b1fb732.png)

**Answer:**

By WLLN, $\bar{X} \overset{P}{\rightarrow} p$

$E(X)=p$ and $Var(X)=p(1-p)$

By CLT,

$\frac{\sqrt{n}(\bar{X}-p)}{\sqrt{p(1-p)}} \overset{D}{\rightarrow} N(0,1)$

Since $\frac{p(1-p)}{\sqrt{\bar{X}(1-\bar{X})}}\overset{P}{\rightarrow}1$

$\frac{\sqrt{n}(\bar{X}-p)}{\sqrt{\bar{X}(1-\bar{X})}} \overset{D}{\rightarrow} N(0,1)$

$P(|\frac{\sqrt{n}(\bar{X}-p)}{\sqrt{\bar{X}(1-\bar{X})}}|\leq 1.96)=0.95$

$P(-1.96\leq \frac{\sqrt{n}(\bar{X}-p)}{\sqrt{\bar{X}(1-\bar{X})}}\leq 1.96)=0.95$

$P(\frac{-1.96\sqrt{\bar{X}(1-\bar{X})}}{\sqrt{n}}\leq \bar{X}-p\leq \frac{1.96\sqrt{\bar{X}(1-\bar{X})}}{\sqrt{n}})=0.95$

$P(\bar{X}-\frac{1.96\sqrt{\bar{X}(1-\bar{X})}}{\sqrt{n}}\leq p\leq \bar{X}+\frac{1.96\sqrt{\bar{X}(1-\bar{X})}}{\sqrt{n}})=0.95$

Hence, 95% asymptotic CI for p is $(\bar{X}-\frac{1.96\sqrt{\bar{X}(1-\bar{X})}}{\sqrt{n}}, \bar{X}+\frac{1.96\sqrt{\bar{X}(1-\bar{X})}}{\sqrt{n}})$

# Question 4

![](images/WeChatced7f5ac7391fba18ddafc0ce9a0786f.png)

![](images/WeChat09fcf42ca2f8c77104c6ae92c715e35c.png){width="167" height="21"}

**Answer:**

Let $N=n+m$, $\gamma$ is Kurtosis of X

By WLLN and C.M.T,

$\sqrt{N}\sqrt{\frac{S_X^2}{n}+\frac{S_Y^2}{m}}=\sqrt{\frac{S_X^2}{n/N}+\frac{S_Y^2}{m/N}}\overset{P}{\rightarrow}\sqrt{\frac{\sigma_X^2}{\gamma}+\frac{\sigma_Y^2}{1-\gamma}}$

$\sqrt{N}\{\bar{X}-\bar{Y}-(\mu_X-\mu_Y)\}=\sqrt{\frac{N}{n}}\sqrt{n}(\bar{X}-\mu_X)-\sqrt{\frac{N}{m}}\sqrt{m}(\bar{Y}-\mu_Y)$

Then,

```{=tex}
\begin{align*}
M(t)&=E(e^{t\sqrt{\frac{N}{n}}\sqrt{n}(\bar{X}-\mu_X)-t\sqrt{\frac{N}{m}}\sqrt{m}(\bar{Y}-\mu_Y)})\\
&=E\{e^{t\sqrt{\frac{N}{n}}\sigma_X\frac{\sqrt{n}(\bar{X}-\mu_X)}{\sigma_X}}\}E\{e^{t\sqrt{\frac{N}{m}}\sigma_Y\frac{\sqrt{m}(\bar{Y}-\mu_Y)}{\sigma_Y}}\}\\
&=M_Z(t\sqrt{\frac{1}{\gamma}}\sigma_X)M_Z(t\sqrt{\frac{1}{1-\gamma}\sigma_Y})\\
&=e^{\frac{t^2}{2}(\frac{\sigma_X^2}{\gamma}+\frac{\sigma_Y^2}{1-\gamma})} \text{,  }\forall t
\end{align*}
```
Hence,

$\sqrt{N}\{\bar{X}-\bar{Y}-(\mu_X-\mu_Y)\}\overset{D}{\rightarrow}N(0,\frac{\sigma_X^2}{\gamma}+\frac{\sigma_Y^2}{1-\gamma})$

By combining the above results,

$\frac{\bar{X}-\bar{Y}-(\mu_X-\mu_Y)}{\sqrt{\frac{S_X^2}{n}+\frac{S_Y^2}{m}}}\overset{D}{\rightarrow}Z\sim N(0,1)$

# Question 5

![](images/WeChat75d07e25c2e1701111d95e3fbd1e123a.png)

**(a) Answer:**

Since $X_i \sim Poisson(\theta)$,

BY WLLN,

$\frac{\sqrt{n}(\bar{X}-\theta)}{\sqrt{\theta}} \overset{D}{\rightarrow} N(0,1)$

$\sqrt{n}\{\bar{X}-\theta\} \overset{D}{\rightarrow} N(0,\theta)$

**(b) Answer:**

By delta method,

$\sqrt{n}\{g(\bar{X})-g(\theta)\} \overset{D}{\rightarrow} N(0,\theta^2(g'(\theta))^2)$

# Question 6

![](images/WeChat4083c7db7d2ba8b7c6e5579d5556c114.png)

![](images/WeChata36ef4caa6ec9b0e8ae8568bb93f21ea.png)

**(a) Answer:**

To ensure $[g'(\theta)]^2\sigma^2(\theta)=1$, we need $g'(\theta)=\frac{1}{\sqrt{\sigma^2}}$

Since $X_1,X_2,...,X_n \overset{\text{i.i.d.}}{\sim} Exponential(\frac{1}{\theta})$

Then, $\sigma^2=\theta^2$

$g'(\theta)=\frac{1}{\sqrt{\theta^2}}=\frac{1}{\theta}$

$g(\theta)=\ln(\theta)$

Hence, $g(X_n)=\ln(X_n)$ is the variance stabilizing transformation.

**(b) Answer:**

Similarly, we need $g'(\theta)=\frac{1}{\sqrt{\sigma^2}}$

Since $X_1,X_2,...,X_n \overset{\text{i.i.d.}}{\sim} Poisson(\theta)$

Then, $\sigma^2=\theta$

$g'(\theta)=\frac{1}{\sqrt{\theta}}$

$g(\theta)=2\sqrt{\theta}$

Hence, $g(X_n)=2\sqrt{X_n}$ is the variance stabilizing transformation.

**(c) Answer:**

Similarly, we need $g'(\theta)=\frac{1}{\sqrt{\sigma^2}}$

Since $X_1,X_2,...,X_n \overset{\text{i.i.d.}}{\sim} Bernoulli(\theta)$

Then, $\sigma^2=\theta(1-\theta)$

$g'(\theta)=\frac{1}{\sqrt{\theta(1-\theta)}}$

$g(\theta)=\arcsin(2\theta-1)$

Hence, $g(X_n)=\arcsin(2X_n-1)$ is the variance stabilizing transformation.

**(d) Answer:**

$\sqrt{n}(X_n-\theta) \overset{D}{\rightarrow} N(0,\sigma^2)$

After transformation, we have

$\sqrt{n}(2\sqrt{X_n}-2\sqrt{\theta}) \overset{D}{\rightarrow} N(0,1)$

$P(-1.96\leq \sqrt{n}(2\sqrt{X_n}-2\sqrt{\theta})\leq 1.96)=0.95$

$P(\frac{-1.96}{\sqrt{n}}\leq 2\sqrt{X_n}-2\sqrt{\theta}\leq\frac{1.96}{\sqrt{n}})=0.95$

$P(\frac{-1.96}{2\sqrt{n}}\leq \sqrt{X_n}-\sqrt{\theta}\leq\frac{1.96}{2\sqrt{n}})=0.95$

$P(\sqrt{X_n}-\frac{1.96}{2\sqrt{n}}\leq \sqrt{\theta}\leq\sqrt{X_n}+\frac{1.96}{2\sqrt{n}})=0.95$

$P((\sqrt{X_n}-\frac{1.96}{2\sqrt{n}})^2\leq \theta\leq(\sqrt{X_n}+\frac{1.96}{2\sqrt{n}})^2)=0.95$
